src/BellCriteriaDecl.v
@@ -1,4 +1,4 @@
-From Stdlib Require Import Arith.
+From Stdlib Require Import PeanoNat.
 From Stdlib Require Import Bool.
 From Stdlib Require Import List.
 From Stdlib Require Import ZArith.
